PKE_Enc and PKE_Dec for Spec.HPKE

specs/experimental/Spec.HPKE.fst
@@ -406,3 +406,34 @@ let setupPSKAuthR cs pkE pkI skR psk pskID info =
 
 /// Encrypt() and Decrypt using the derived AEAD key and nonce
 /// are implemented by calling AEAD.encrypt and AEAD.Decrypt
+
+val encryptBase:
+    cs:ciphersuite
+  -> skE:key_dh_secret_s cs
+  -> pkR:key_dh_public_s cs
+  -> m:bytes
+  -> info:bytes{Seq.length info <= max_info} ->
+  Tot (option bytes)
+
+let encryptBase cs skE pkR m info =
+  let zz, pkR = encap cs skE pkR in
+  let pkE,k,n = setupBaseI cs skE pkR info in
+  match Spec.Defensive.AEAD.encrypt (aead_of_cs cs) k n m info with
+  | None -> None
+  | Some c -> Some (Seq.append pkE c)
+
+
+val decryptBase:
+    cs:ciphersuite
+  -> pkE:key_dh_public_s cs
+  -> skR:key_dh_secret_s cs
+  -> input:bytes{size_dh_public cs <= Seq.length input /\ Seq.length input <= max_size_t}
+  -> info:bytes{Seq.length info <= max_info} ->
+  Tot (option bytes)
+
+let decryptBase cs pkE skR input info =
+  let pkE = sub #uint8 #(Seq.length input) input 0 (size_dh_key cs) in
+  let c = sub #uint8 #(Seq.length input) input (size_dh_public cs) (length input - (size_dh_public cs)) in
+  let zz = decap cs pkE skR in
+  let k,n = setupBaseR cs pkE skR info in
+  Spec.Defensive.AEAD.decrypt (aead_of_cs cs) k n c info
